refactoring

Auto/Embedding/LCtx.lean
@@ -1,372 +1,515 @@
 import Auto.Util.HEqExtra
+import Std.Data.Nat.Lemmas
 namespace Auto.Embedding
 
-@[reducible] def pushLCtx (lctx : Nat → α) (x : α) : Nat → α
-| 0     => x
-| n + 1 => lctx n
+section push
+  
+  def pushLCtxAt (x : α) (pos : Nat) (lctx : Nat → α) (n : Nat) : α :=
+    match n.ble pos with
+    | true => 
+      match n.beq pos with
+      | true => x
+      | false => lctx n
+    | false => lctx (.pred n)
+  
+  theorem pushLCtxAt.succ_zero (x : α) (pos : Nat) (lctx : Nat → α) :
+    pushLCtxAt x (.succ pos) lctx 0 = lctx 0 := rfl
+  
+  theorem pushLCtxAt.succ_succ (x : α) (pos : Nat) (lctx : Nat → α) (n : Nat) :
+    pushLCtxAt x (.succ pos) lctx (.succ n) = pushLCtxAt x pos (fun n => lctx (.succ n)) n := by
+    dsimp [pushLCtxAt, Nat.ble, Nat.beq];
+    match h : Nat.ble n pos with
+    | true => rfl
+    | false =>
+      dsimp; cases n;
+      case zero =>
+        have h' : Nat.ble Nat.zero pos = true :=
+          Nat.ble_eq_true_of_le (Nat.zero_le _)
+        rw [h] at h'; cases h'
+      case succ n' => rfl
+  
+  theorem pushLCtxAt.succ_succ_Fn (x : α) (pos : Nat) (lctx : Nat → α) :
+    (fun n => pushLCtxAt x (.succ pos) lctx (.succ n)) = pushLCtxAt x pos (fun n => lctx (.succ n)) :=
+    funext (fun n => pushLCtxAt.succ_succ x pos lctx n)
+  
+  def pushLCtxAt.comm (f : α → β) (x : α) (pos : Nat) (lctx : Nat → α) (n : Nat) :
+    f (pushLCtxAt x pos lctx n) = pushLCtxAt (f x) pos (f ∘ lctx) n := by
+    dsimp [pushLCtxAt]
+    match n.ble pos with
+    | true =>
+      match n.beq pos with
+      | true => rfl
+      | false => rfl
+    | false => rfl
+  
+  theorem pushLCtxAt.commFn (f : α → β) (x : α) (pos : Nat) (lctx : Nat → α) :
+    (fun n => f (pushLCtxAt x pos lctx n)) = (fun n => pushLCtxAt (f x) pos (fun n => f (lctx n)) n) :=
+    funext (pushLCtxAt.comm f x pos lctx)
+  
+  def pushLCtxAtDep
+    {rty : Nat → α} {lctxty : α → Sort u} {xty : α} (x : lctxty xty) (pos : Nat)
+    (lctx : ∀ n, lctxty (rty n)) (n : Nat) : lctxty (pushLCtxAt xty pos rty n) := by
+    dsimp [pushLCtxAt]
+    match n.ble pos with
+    | true =>
+      match n.beq pos with
+      | true => exact x
+      | false => exact (lctx n)
+    | false => exact (lctx (.pred n))
+  
+  theorem pushLCtxAtDep.succ_zero {rty : Nat → α} {lctxty : α → Sort u}
+    {xty : α} (x : lctxty xty) (pos : Nat) (lctx : ∀ n, lctxty (rty n)) :
+    pushLCtxAtDep x (.succ pos) lctx 0 = lctx 0 := rfl
+  
+  theorem pushLCtxAtDep.succ_succ {rty : Nat → α} {lctxty : α → Sort u} {xty : α}
+    (x : lctxty xty) (pos : Nat) (lctx : ∀ n, lctxty (rty n)) (n : Nat) :
+    HEq (pushLCtxAtDep x (.succ pos) lctx (.succ n)) (pushLCtxAtDep x pos (fun n => lctx (.succ n)) n) := by
+    dsimp [pushLCtxAt, pushLCtxAtDep, Nat.ble, Nat.beq]
+    match h : Nat.ble n pos with
+    | true => rfl
+    | false =>
+      dsimp; cases n;
+      case zero =>
+        have h' : Nat.ble Nat.zero pos = true :=
+          Nat.ble_eq_true_of_le (Nat.zero_le _)
+        rw [h] at h'; cases h'
+      case succ n' => rfl
+  
+  theorem pushLCtxAtDep.succ_succ_Fn {rty : Nat → α} {lctxty : α → Sort u}
+    {xty : α} (x : lctxty xty) (pos : Nat) (lctx : ∀ n, lctxty (rty n)) :
+    HEq (fun n => pushLCtxAtDep x (.succ pos) lctx (.succ n)) (pushLCtxAtDep x pos (fun n => lctx (.succ n))) :=
+    HEq.funext _ _ (fun n => pushLCtxAtDep.succ_succ x pos lctx n)
+  
+  def pushLCtxAtDep.comm {α : Sort w} {β : α → Sort x} {rty : Nat → α} {lctxty : α → Sort u}
+    (f : ∀ (x : α), lctxty x → β x) {xty : α} (x : lctxty xty) (pos : Nat)
+    (lctx : ∀ n, lctxty (rty n)) (n : Nat) :
+      f _ (pushLCtxAtDep x pos lctx n) = pushLCtxAtDep (lctxty:=β) (f xty x) pos (fun n => f _ (lctx n)) n := by
+    dsimp [pushLCtxAt, pushLCtxAtDep]
+    match n.ble pos with
+    | true =>
+      match n.beq pos with
+      | true => rfl
+      | false => rfl
+    | false => rfl
+  
+  def pushLCtxAtDep.nonDep {rty : Nat → α} {lctxty : Sort u}
+    {xty : α} (x : lctxty) (pos : Nat) (lctx : Nat → lctxty) (n : Nat) :
+    @pushLCtxAtDep _ rty (fun _ => lctxty) xty x pos lctx n = pushLCtxAt x pos lctx n := rfl
+  
+  def pushLCtxAtDep.absorbAux {rty : Nat → α} {lctxty : α → Sort u}
+    {xty : α} (x : lctxty xty) (pos : Nat) (lctx : ∀ n, lctxty (rty n)) (n : Nat) :
+    HEq
+      (@pushLCtxAtDep _ rty lctxty _ x pos lctx n)
+      (@pushLCtxAtDep _ (lctxty ∘ rty) id _ x pos lctx n) := by
+    dsimp [pushLCtxAt, pushLCtxAtDep]
+    match n.ble pos with
+    | true =>
+      match n.beq pos with
+      | true => apply HEq.rfl
+      | false => apply HEq.rfl
+    | false => apply HEq.rfl
+  
+  theorem pushLCtxAtDep.absorb {rty : Nat → α} {lctxty : α → Sort u}
+    {xty : α} (x : lctxty xty) (pos : Nat) (lctx : ∀ n, lctxty (rty n)) :
+    HEq (@pushLCtxAtDep _ rty lctxty _ x pos lctx) (@pushLCtxAtDep _ (lctxty ∘ rty) id _ x pos lctx) :=
+    HEq.funext _ _ (pushLCtxAtDep.absorbAux _ _ _)
+  
+  @[reducible] def pushLCtx (x : α) (lctx : Nat → α) := pushLCtxAt x 0 lctx
+  
+  def pushLCtx.zero (x : α) (lctx : Nat → α) : pushLCtx x lctx 0 = x := rfl
+  
+  def pushLCtx.succ (x : α) (lctx : Nat → α) (n : Nat) : pushLCtx x lctx (.succ n) = lctx n := rfl
+  
+  def pushLCtx.succ_Fn (x : α) (lctx : Nat → α) :
+    (fun n => pushLCtx x lctx (.succ n)) = lctx := rfl
 
-def pushLCtx.comm (f : α → β) (lctx : Nat → α) (x : α) :
-  (n : Nat) → f (pushLCtx lctx x n) = pushLCtx (fun n => f (lctx n)) (f x) n
-| 0       => rfl
-| .succ _ => rfl
+  theorem pushLCtxAt.zero (x : α) (lctx : Nat → α) (n : Nat) :
+    pushLCtxAt x 0 lctx n = pushLCtx x lctx n := rfl
+  
+  def pushLCtx.comm (f : α → β) (x : α) (lctx : Nat → α) (n : Nat) :
+    f (pushLCtx x lctx n) = pushLCtx (f x) (fun n => f (lctx n)) n :=
+    pushLCtxAt.comm f x 0 lctx n
+  
+  theorem pushLCtx.commFn (f : α → β) (x : α) (lctx : Nat → α) :
+    (fun n => f (pushLCtx x lctx n)) = (fun n => pushLCtx (f x) (fun n => f (lctx n)) n) :=
+    funext (pushLCtx.comm f x lctx)
+  
+  def pushLCtx_pushLCtxAt (x y : α) (pos : Nat) (lctx : Nat → α) :
+    pushLCtx y (pushLCtxAt x pos lctx) = pushLCtxAt x (Nat.succ pos) (pushLCtx y lctx) := by
+    apply funext; intro n; cases n; rfl; rw [pushLCtxAt.succ_succ]; rfl
+  
+  @[reducible] def pushLCtxDep {rty : Nat → α} {lctxty : α → Sort u}
+    {xty : α} (x : lctxty xty) (lctx : ∀ n, lctxty (rty n)) := pushLCtxAtDep x 0 lctx
+  
+  def pushLCtxDep.zero {rty : Nat → α} {lctxty : α → Sort u}
+    {xty : α} (x : lctxty xty) (lctx : ∀ n, lctxty (rty n)) :
+    pushLCtxDep x lctx 0 = x := rfl
+  
+  def pushLCtxDep.succ {rty : Nat → α} {lctxty : α → Sort u}
+    (lctx : ∀ n, lctxty (rty n)) {xty : α} (x : lctxty xty) (n : Nat) :
+    pushLCtxDep x lctx (.succ n) = lctx n := rfl
 
-theorem pushLCtx.commFn (f : α → β) (lctx : Nat → α) (x : α) :
-  (fun n => f (pushLCtx lctx x n)) = (fun n => pushLCtx (fun n => f (lctx n)) (f x) n) :=
-  funext (pushLCtx.comm f lctx x)
+  def pushLCtxDep.succ_Fn {rty : Nat → α} {lctxty : α → Sort u}
+    (lctx : ∀ n, lctxty (rty n)) {xty : α} (x : lctxty xty) :
+    (fun n => pushLCtxDep x lctx (.succ n)) = lctx := rfl
+  
+  theorem pushLCtxAtDep.zero {rty : Nat → α} {lctxty : α → Sort u}
+    (lctx : ∀ n, lctxty (rty n)) {xty : α} (x : lctxty xty) (n : Nat) :
+    pushLCtxAtDep x 0 lctx n = pushLCtxDep x lctx n := rfl
+  
+  def pushLCtxDep.comm {α : Sort w} {β : α → Sort x} {rty : Nat → α} {lctxty : α → Sort u}
+    (f : ∀ (x : α), lctxty x → β x) (lctx : ∀ n, lctxty (rty n))
+    {xty : α} (x : lctxty xty) (n : Nat) :
+    f _ (pushLCtxDep x lctx n) = pushLCtxDep (lctxty:=β) (f xty x) (fun n => f _ (lctx n)) n :=
+    pushLCtxAtDep.comm f x 0 lctx n
+  
+  def pushLCtxDep.absorbAux {rty : Nat → α} {lctxty : α → Sort u}
+    (lctx : ∀ n, lctxty (rty n)) {xty : α} (x : lctxty xty) (n : Nat) :
+    HEq
+      (@pushLCtxDep _ rty lctxty _ x lctx n)
+      (@pushLCtxDep _ (lctxty ∘ rty) id _ x lctx n) :=
+    pushLCtxAtDep.absorbAux x 0 lctx n
+  
+  theorem pushLCtxDep.absorb {rty : Nat → α} {lctxty : α → Sort u}
+    (lctx : ∀ n, lctxty (rty n)) {xty : α} (x : lctxty xty) :
+    HEq (@pushLCtxDep _ rty lctxty _ x lctx) (@pushLCtxDep _ (lctxty ∘ rty) id _ x lctx) :=
+    pushLCtxAtDep.absorb x 0 lctx
+  
+  -- Surprisingly, this is definitionally equal
+  def pushLCtxDep_pushLCtxAtDep {rty : Nat → α} {lctxty : α → Sort u}
+    (lctx : ∀ n, lctxty (rty n)) {xty : α} (x : lctxty xty) {yty : α} (y : lctxty yty) (pos : Nat) :
+    HEq (pushLCtxDep y (pushLCtxAtDep x pos lctx)) (pushLCtxAtDep x (Nat.succ pos) (pushLCtxDep y lctx)) := by
+    apply HEq.funext; intro n; cases n; rfl;
+    apply HEq.trans _ (HEq.symm (pushLCtxAtDep.succ_succ _ _ _ _)); apply HEq.rfl
+  
+  @[reducible] def pushLCtxs (xs : List α) (lctx : Nat → α) (n : Nat) : α :=
+    match h : Nat.blt n xs.length with
+    | true  => xs[n]'(Nat.le_of_ble_eq_true h)
+    | false => lctx (n - xs.length)
 
-@[reducible] def pushLCtxDep {rty : Nat → α} {lctxty : α → Sort u}
-  (lctx : ∀ n, lctxty (rty n)) {xty : α} (x : lctxty xty) : ∀ n, lctxty (pushLCtx rty xty n)
-| 0     => x
-| n + 1 => lctx n
+end push
 
-def pushLCtxDep.comm {α : Sort w} {β : α → Sort x} {rty : Nat → α} {lctxty : α → Sort u}
-  (f : ∀ (x : α), lctxty x → β x) (lctx : ∀ n, lctxty (rty n))
-  {xty : α} (x : lctxty xty) : (n : Nat) →
-  f _ (pushLCtxDep lctx x n) = pushLCtxDep (lctxty:=β) (fun n => f _ (lctx n)) (f xty x) n
-| 0 => rfl
-| _ + 1  => rfl
 
-def pushLCtxDep.absorbAux {rty : Nat → α} {lctxty : α → Sort u}
-  (lctx : ∀ n, lctxty (rty n)) {xty : α} (x : lctxty xty) :
-  (n : Nat) → HEq
-    (@pushLCtxDep _ rty lctxty lctx _ x n)
-    (@pushLCtxDep _ (lctxty ∘ rty) id lctx _ x n)
-| 0 => HEq.refl _
-| _ + 1 => HEq.refl _
-
-theorem pushLCtxDep.absorb {rty : Nat → α} {lctxty : α → Sort u}
-  (lctx : ∀ n, lctxty (rty n)) {xty : α} (x : lctxty xty) :
-  HEq (@pushLCtxDep _ rty lctxty lctx _ x) (@pushLCtxDep _ (lctxty ∘ rty) id lctx _ x) :=
-  HEq.funext _ _ (pushLCtxDep.absorbAux _ _)
-
-def pushLCtxAt (lctx : Nat → α) (x : α) (pos n : Nat) : α :=
-  match n.ble pos with
-  | true => 
-    match n.beq pos with
-    | true => x
+section pop
+  
+  def popLCtxAt (pos : Nat) (lctx : Nat → α) (n : Nat) :=
+    match pos.ble n with
+    | true => lctx (.succ n)
     | false => lctx n
-  | false => lctx (.pred n)
+  
+  theorem popLCtxAt.succ_zero (pos : Nat) (lctx : Nat → α) :
+    popLCtxAt (.succ pos) lctx 0 = lctx 0 := rfl
+  
+  theorem popLCtxAt.succ_succ (pos : Nat) (lctx : Nat → α) (n : Nat) :
+    popLCtxAt (.succ pos) lctx (.succ n) = popLCtxAt pos (fun n => lctx (.succ n)) n := rfl
+  
+  def popLCtxAt.comm (f : α → β) (pos : Nat) (lctx : Nat → α) (n : Nat) :
+    f (popLCtxAt pos lctx n) = popLCtxAt pos (f ∘ lctx) n := by
+    dsimp [popLCtxAt]
+    match pos.ble n with
+    | true => rfl
+    | false => rfl
+  
+  def popLCtxAt.commFn (f : α → β) (pos : Nat) (lctx : Nat → α) :
+    (fun n => f (popLCtxAt pos lctx n)) = (fun n => popLCtxAt pos (f ∘ lctx) n) :=
+    funext (popLCtxAt.comm f pos lctx)
+  
+  def popLCtxAtDep {rty : Nat → α} {lctxty : α → Sort u}
+    (pos : Nat) (lctx : ∀ n, lctxty (rty n)) (n : Nat) : lctxty (popLCtxAt pos rty n) := by
+    dsimp [popLCtxAt]
+    match pos.ble n with
+    | true => exact lctx (.succ n)
+    | false => exact lctx n
+  
+  theorem popLCtxAtDep.succ_zero {rty : Nat → α} {lctxty : α → Sort u}
+    (lctx : ∀ n, lctxty (rty n)) (pos : Nat) :
+    popLCtxAtDep (.succ pos) lctx 0 = lctx 0 := rfl
+  
+  theorem popLCtxAtDep.succ_succ {rty : Nat → α} {lctxty : α → Sort u}
+    (pos : Nat) (lctx : ∀ n, lctxty (rty n)) (n : Nat) :
+    popLCtxAtDep (.succ pos) lctx (.succ n) = popLCtxAtDep pos (fun n => lctx (.succ n)) n := rfl
+  
+  def popLCtxAtDep.absorbAux {rty : Nat → α} {lctxty : α → Sort u}
+    (pos : Nat) (lctx : ∀ n, lctxty (rty n)) (n : Nat) : HEq
+      (@popLCtxAtDep _ rty lctxty pos lctx n)
+      (@popLCtxAtDep _ (lctxty ∘ rty) id pos lctx n) := by
+    dsimp [popLCtxAt, popLCtxAtDep]
+    match pos.ble n with
+    | true => rfl
+    | false => rfl
+  
+  def popLCtxAtDep.absorbAux' {rty : Nat → α} {lctxty : α → Sort u}
+    (pos : Nat) (lctx : ∀ n, lctxty (rty n)) (n : Nat) : HEq
+      (@popLCtxAtDep _ rty lctxty pos lctx n)
+      (@popLCtxAtDep _ id (lctxty ∘ rty) pos lctx n) :=
+    HEq.trans
+      (b := @popLCtxAtDep _ (lctxty ∘ rty) id pos lctx n)
+      (popLCtxAtDep.absorbAux pos lctx n)
+      (HEq.symm (@popLCtxAtDep.absorbAux _ id (lctxty ∘ rty) pos lctx n))
+  
+  def popLCtxAtDep.absorb {rty : Nat → α} {lctxty : α → Sort u} (pos : Nat) (lctx : ∀ n, lctxty (rty n)):
+    HEq (@popLCtxAtDep _ rty lctxty pos lctx) (@popLCtxAtDep _ (lctxty ∘ rty) id pos lctx) :=
+    HEq.funext _ _ (popLCtxAtDep.absorbAux _ _)
+  
+  def popLCtxAtDep.comm {α : Sort w} {β : α → Sort x} {rty : Nat → α} {lctxty : α → Sort u}
+    (f : ∀ (x : α), lctxty x → β x) (pos : Nat) (lctx : ∀ n, lctxty (rty n)) (n : Nat) :
+      f _ (popLCtxAtDep pos lctx n) = popLCtxAtDep (lctxty:=β) pos (fun n => f _ (lctx n)) n := by
+    dsimp [popLCtxAt, popLCtxAtDep]
+    match pos.ble n with
+    | true => rfl
+    | false => rfl
+  
+  def popLCtxAtDep.commFn {α : Sort w} {β : α → Sort x} {rty : Nat → α} {lctxty : α → Sort u}
+    (f : ∀ (x : α), lctxty x → β x) (pos : Nat) (lctx : ∀ n, lctxty (rty n)) :
+    (fun n => f _ (popLCtxAtDep pos lctx n)) = (fun n => popLCtxAtDep (lctxty:=β) pos (fun n => f _ (lctx n)) n) :=
+    funext (fun n => popLCtxAtDep.comm f pos lctx n)
+  
+  def popLCtxAt.commDep
+    {β : α → Sort u} (f : ∀ (x : α), β x) (pos : Nat) (lctx : Nat → α) (n : Nat) :
+      f (popLCtxAt pos lctx n) = popLCtxAtDep pos (fun n => f (lctx n)) n := by
+    dsimp [popLCtxAt, popLCtxAtDep]
+    match pos.ble n with
+    | true => rfl
+    | false => rfl
 
-def pushLCtxAtRec (lctx : Nat → α) (x : α) : (pos : Nat) → Nat → α
-| 0 => pushLCtx lctx x
-| pos' + 1 => fun n =>
-  match n with
-  | 0 => lctx 0
-  | n' + 1 => pushLCtxAtRec (fun n => lctx (Nat.succ n)) x pos' n'
+  def popLCtx (lctx : Nat → α) := popLCtxAt 0 lctx
+  
+  def popLCtx.comm (f : α → β) (lctx : Nat → α) (n : Nat) :
+    f (popLCtx lctx n) = popLCtx (f ∘ lctx) n := popLCtxAt.comm f 0 lctx n
+  
+  def popLCtx.commFn (f : α → β) (lctx : Nat → α) :
+    (fun n => f (popLCtx lctx n)) = (fun n => popLCtx (f ∘ lctx) n) :=
+    popLCtxAt.commFn f 0 lctx
+  
+  def popLCtxDep {rty : Nat → α} {lctxty : α → Sort u}
+    (lctx : ∀ n, lctxty (rty n)) : ∀ n, lctxty (popLCtx rty n) :=
+    popLCtxAtDep 0 lctx
+  
+  def popLCtxDep.comm {α : Sort w} {β : α → Sort x} {rty : Nat → α} {lctxty : α → Sort u}
+    (f : ∀ (x : α), lctxty x → β x) (lctx : ∀ n, lctxty (rty n)) (n : Nat) :
+    f _ (popLCtxDep lctx n) = popLCtxDep (lctxty:=β) (fun n => f _ (lctx n)) n :=
+    popLCtxAtDep.comm f 0 lctx n
+  
+  def popLCtxDep.absorbAux {rty : Nat → α} {lctxty : α → Sort u}
+    (lctx : ∀ n, lctxty (rty n)) (n : Nat) : HEq
+      (@popLCtxDep _ rty lctxty lctx n)
+      (@popLCtxDep _ (lctxty ∘ rty) id lctx n) :=
+      popLCtxAtDep.absorbAux 0 lctx n
+  
+  theorem popLCtxDep.absorb {rty : Nat → α} {lctxty : α → Sort u} (lctx : ∀ n, lctxty (rty n)) :
+    HEq (@popLCtxDep _ rty lctxty lctx) (@popLCtxDep _ (lctxty ∘ rty) id lctx) :=
+    popLCtxAtDep.absorb 0 lctx
+  
+  def popLCtxsAt (lvl pos : Nat) (lctx : Nat → α) (n : Nat) :=
+    match pos.ble n with
+    | true => lctx (Nat.add n lvl)
+    | false => lctx n
+  
+  def popLCtxsAt.comm (f : α → β) (lvl pos : Nat) (lctx : Nat → α) (n : Nat) :
+    f (popLCtxsAt lvl pos lctx n) = popLCtxsAt lvl pos (f ∘ lctx) n := by
+    dsimp [popLCtxsAt]
+    match Nat.ble pos n with
+    | true => rfl
+    | false => rfl
+  
+  def popLCtxsAt.succ_l (lvl pos : Nat) (lctx : Nat → α) (n : Nat) :
+    popLCtxsAt (.succ lvl) pos lctx n = popLCtxsAt lvl pos (popLCtxAt pos lctx) n := by
+    dsimp [popLCtxsAt, popLCtxAt]
+    match h : Nat.ble pos n with
+    | true =>
+      dsimp
+      have leAdd' := Nat.le_trans (Nat.le_of_ble_eq_true h) (Nat.le_add_right _ lvl)
+      have bleAdd' := Nat.ble_eq_true_of_le leAdd'
+      rw [bleAdd']; rfl
+    | false => rfl
+  
+  def popLCtxsAt.succ_r (lvl pos : Nat) (lctx : Nat → α) (n : Nat) :
+    popLCtxsAt (.succ lvl) pos lctx n = popLCtxAt pos (popLCtxsAt lvl pos lctx) n := by
+    dsimp [popLCtxsAt, popLCtxAt]
+    match h : Nat.ble pos n with
+    | true =>
+      dsimp
+      dsimp
+      have leAdd' := Nat.le_trans (Nat.le_of_ble_eq_true h) (Nat.le_add_right _ 1)
+      have bleAdd' := Nat.ble_eq_true_of_le leAdd'
+      rw [bleAdd', Nat.succ_add]; rfl
+    | false => rfl
+  
+  def popLCtxsAt.one (pos : Nat) (lctx : Nat → α) :
+    popLCtxsAt 1 pos lctx = popLCtxAt pos lctx := rfl
 
-def pushLCtxAt.equiv (lctx : Nat → α) (x : α) (pos n : Nat) :
-  pushLCtxAtRec lctx x pos n = pushLCtxAt lctx x pos n := by
-  revert lctx n; induction pos <;> intro lctx n
-  case zero =>
-    cases n <;> rfl
-  case succ pos' IH =>
-    cases n
+end pop
+
+
+section push_pop
+
+  def push_pop_eq (lctx : Nat → α) :
+    pushLCtx (lctx 0) (popLCtx lctx) = lctx := by
+    apply funext
+    intro n; cases n
     case zero => rfl
-    case succ n' =>
-      let IH' := IH (fun n => lctx (.succ n)) n'
-      dsimp [pushLCtxAtRec, pushLCtxAt, Nat.ble, Nat.beq]
-      dsimp [pushLCtxAtRec, pushLCtxAt, Nat.ble, Nat.beq] at IH'
-      cases n'
-      case zero =>
-        rw [Nat.ble_eq_true_of_le (Nat.zero_le _)]; dsimp
-        rw [Nat.ble_eq_true_of_le (Nat.zero_le _)] at IH'; dsimp at IH'
-        exact IH'
-      case succ n' =>
-        exact IH'
+    case succ n' => cases n' <;> rfl    
+  
+  def popAt_pushAt_eq (x : α) (pos : Nat) (lctx : Nat → α) (n : Nat) :
+    popLCtxAt pos (pushLCtxAt x pos lctx) n = lctx n :=
+    match pos, n with
+    | 0, 0       => rfl
+    | 0, .succ _ => rfl
+    | .succ _, 0 => rfl
+    | .succ pos' , .succ n' => by
+      rw [popLCtxAt.succ_succ]; rw [pushLCtxAt.succ_succ_Fn];
+      exact (popAt_pushAt_eq x pos' (fun n => lctx (.succ n)) n')
+  
+  def popAtDep_pushAtDep_eq
+    {α : Sort w} {rty : Nat → α} {lctxty : α → Sort u}
+    {xty : α} (x : lctxty xty) (pos : Nat) (lctx : ∀ n, lctxty (rty n)) (n : Nat) :
+    HEq
+      (@popLCtxAtDep _ (pushLCtxAt xty pos rty) lctxty
+        pos (@pushLCtxAtDep _ rty lctxty xty x pos lctx) n)
+      (lctx n) :=
+    match pos, n with
+    | 0, 0       => HEq.rfl
+    | 0, .succ _ => HEq.rfl
+    | .succ _, 0 => HEq.rfl
+    | .succ pos' , .succ n' => by
+      apply HEq.trans (heq_of_eq (popLCtxAtDep.succ_succ _ _ _))
+      apply HEq.trans _ (popAtDep_pushAtDep_eq x pos' (fun n => lctx (.succ n)) n')
+      apply (congr_arg₂_heq
+        (γ := fun rty _ => lctxty (popLCtxAt pos' rty n'))
+        (fun rty lctx => popLCtxAtDep (rty:=rty) pos' lctx n') _ _)
+      apply pushLCtxAt.succ_succ_Fn
+      apply pushLCtxAtDep.succ_succ_Fn
 
-theorem pushLCtxAt.equivFn (lctx : Nat → α) (x : α) (pos : Nat) :
-  pushLCtxAtRec lctx x pos = pushLCtxAt lctx x pos :=
-  funext (fun n => pushLCtxAt.equiv lctx x pos n)
+end push_pop
 
-def pushLCtxAtRec.comm (f : α → β) (lctx : Nat → α) (x : α) :
-  (pos : Nat) → (n : Nat) → f (pushLCtxAtRec lctx x pos n) = pushLCtxAtRec (f ∘ lctx) (f x) pos n
-| 0 => fun n => by
-  dsimp [pushLCtxAtRec]; apply pushLCtx.comm
-| pos' + 1 => fun n =>
-  match n with
-  | 0 => rfl
-  | n' + 1 => pushLCtxAtRec.comm f (fun n => lctx (Nat.succ n)) x pos' n'
 
-theorem pushLCtxAtRec.commFn (lctx : Nat → α) (f : α → β) (x : α) (pos : Nat) :
-  (fun n => f (pushLCtxAtRec lctx x pos n)) = (fun n => pushLCtxAtRec (fun n => f (lctx n)) (f x) pos n) :=
-  funext (pushLCtxAtRec.comm f lctx x pos)
+section generic
 
--- Surprisingly, this is definitionally equal
-def pushLCtx_pushLCtxAtRec (lctx : Nat → α) (x y : α) (pos : Nat) :
-  pushLCtx (pushLCtxAtRec lctx x pos) y = pushLCtxAtRec (pushLCtx lctx y) x (Nat.succ pos)
-  := rfl
+  def mapAt (pos : Nat) (f : Nat → Nat) (n : Nat) :=
+    match pos.ble n with
+    | true => f (n - pos) + pos
+    | false => n
+  
+  def restoreAt (pos : Nat) (restore : ∀ {α}, (Nat → α) → (Nat → α)) :=
+    fun {α} (lctx : Nat → α) (n : Nat) =>
+      match pos.ble n with
+      | true => restore (fun i => lctx (i + pos)) (n - pos)
+      | false => lctx n
 
-def pushLCtxAtDep {rty : Nat → α} {lctxty : α → Sort u}
-  (lctx : ∀ n, lctxty (rty n)) {xty : α} (x : lctxty xty) (pos n : Nat) : lctxty (pushLCtxAt rty xty pos n) := by
-  dsimp [pushLCtxAt]
-  match n.ble pos with
-  | true =>
-    match n.beq pos with
-    | true => exact x
+  theorem restoreAt.succ_succ (pos : Nat) (restore : ∀ {α}, (Nat → α) → (Nat → α))
+    {α} (lctx : Nat → α) (n : Nat) :
+    restoreAt (.succ pos) restore lctx (.succ n) = restoreAt pos restore (fun n => lctx (.succ n)) n := by
+    dsimp [restoreAt, Nat.ble]; rw [Nat.succ_sub_succ]; rfl
+
+  theorem restoreAt.succ_pushLCtx (restore : ∀ {α}, (Nat → α) → (Nat → α))
+    (x : α) (pos : Nat) (lctx : Nat → α) (n : Nat) :
+    restoreAt (.succ pos) restore (pushLCtx x lctx) n = pushLCtx x (restoreAt pos restore lctx) n :=
+    match pos, n with
+    | 0,          0        => rfl
+    | 0,          .succ _  => rfl
+    | .succ _,    0        => rfl
+    | .succ pos', .succ n' => by
+      rw [restoreAt.succ_succ]
+      rw [pushLCtx.succ, pushLCtx.succ_Fn]
+
+  theorem restoreAt.succ_pushLCtx_Fn (restore : ∀ {α}, (Nat → α) → (Nat → α))
+    (x : α) (pos : Nat) (lctx : Nat → α) :
+    restoreAt (.succ pos) restore (pushLCtx x lctx) = pushLCtx x (restoreAt pos restore lctx) :=
+    funext (fun n => restoreAt.succ_pushLCtx restore x pos lctx n)
+
+  def covPair (f : Nat → Nat) (restore : ∀ {α}, (Nat → α) → (Nat → α)) :=
+    ∀ {α} (lctx : Nat → α) (n : Nat), (restore lctx) (f n) = lctx n
+  
+  def covPairAt (f : Nat → Nat) (restore : ∀ {α}, (Nat → α) → (Nat → α)) :=
+    ∀ {α} (pos : Nat) (lctx : Nat → α) (n : Nat),
+      (restoreAt pos restore lctx) (mapAt pos f n) = lctx n
+  
+  theorem covPairAt.ofCovPair (cp : covPair f restore) : covPairAt f restore := by
+    intros α pos lctx n;
+    dsimp [restoreAt, mapAt]
+    match h : pos.ble n with
+    | true =>
+      dsimp;
+      have heq : Nat.ble pos (f (n - pos) + pos) = true := by
+        apply Nat.ble_eq_true_of_le;
+        apply Nat.le_add_left
+      rw [heq]; dsimp
+      rw [Nat.add_sub_assoc]; rw [Nat.sub_self]; dsimp
+      rw [cp]; rw [Nat.sub_add_cancel (Nat.le_of_ble_eq_true h)]
+      constructor
+    | false => dsimp; rw [h]
+
+  def restoreAtDep (pos : Nat) {restore : ∀ {α}, (Nat → α) → (Nat → α)}
+    (restoreDep : ∀ {rty : Nat → α} {lctxty : α → Sort u}, (∀ n, lctxty (rty n)) → ∀ n, lctxty (restore rty n))
+    {rty : Nat → α} {lctxty : α → Sort u} (lctx : ∀ n, lctxty (rty n)) (n : Nat) : lctxty (restoreAt pos restore rty n) := by
+    dsimp [restoreAt]
+    match Nat.ble pos n with
+    | true  => exact (restoreDep (fun i => lctx (i + pos)) (n - pos))
     | false => exact (lctx n)
-  | false => exact (lctx (.pred n))
 
-def pushLCtxAtDepRec {rty : Nat → α} {lctxty : α → Sort u}
-  (lctx : ∀ n, lctxty (rty n)) {xty : α} (x : lctxty xty) : (pos : Nat) → (n : Nat) → lctxty (pushLCtxAtRec rty xty pos n)
-| 0 => pushLCtxDep lctx x
-| pos' + 1 => fun n =>
-  match n with
-  | 0 => lctx 0
-  | n' + 1 => pushLCtxAtDepRec (fun n => lctx (Nat.succ n)) x pos' n'
+  theorem restoreAtDep.succ_succ (pos : Nat) {restore : ∀ {α}, (Nat → α) → (Nat → α)}
+    (restoreDep : ∀ {α} {rty : Nat → α} {lctxty : α → Sort u}, (∀ n, lctxty (rty n)) → ∀ n, lctxty (restore rty n))
+    {rty : Nat → α} {lctxty : α → Sort u} (lctx : ∀ n, lctxty (rty n)) (n : Nat) :
+    HEq (restoreAtDep (.succ pos) restoreDep lctx (.succ n)) (restoreAtDep pos restoreDep (fun n => lctx (.succ n)) n) := by
+    dsimp [restoreAt, restoreAtDep, Nat.ble]; rw [Nat.succ_sub_succ]; rfl
 
-def pushLCtxAtDep.equiv {rty : Nat → α} {lctxty : α → Sort u}
-  (lctx : ∀ n, lctxty (rty n)) {xty : α} (x : lctxty xty) (pos n : Nat) :
-  HEq (pushLCtxAtDepRec lctx x pos n) (pushLCtxAtDep lctx x pos n) := by
-  dsimp [pushLCtxAtDep, pushLCtxAt];
-  revert rty lctx n; induction pos <;> intro rty lctx n
-  case zero =>
-    cases n <;> apply HEq.refl
-  case succ pos' IH =>
-    cases n
-    case zero => apply HEq.rfl
-    case succ n' =>
-      let IH' := IH (fun n => lctx (.succ n)) n'
-      dsimp [pushLCtxAtDepRec, pushLCtxAtRec, Nat.ble, Nat.beq]
-      dsimp [pushLCtxAtDepRec, pushLCtxAtRec, Nat.ble, Nat.beq] at IH'
-      cases n'
-      case zero =>
-        rw [Nat.ble_eq_true_of_le (Nat.zero_le _)]; dsimp
-        rw [Nat.ble_eq_true_of_le (Nat.zero_le _)] at IH'; dsimp at IH'
-        exact IH'
-      case succ n' =>
-        exact IH'
+  theorem restoreAtDep.succ_pushLCtxDep
+    (restore : ∀ {α}, (Nat → α) → (Nat → α))
+    (restoreDep : ∀ {α} {rty : Nat → α} {lctxty : α → Sort u}, (∀ n, lctxty (rty n)) → ∀ n, lctxty ((restore rty) n))
+    {rty : Nat → α} {lctxty : α → Sort u} {xty : α} (x : lctxty xty) (pos : Nat)
+    (lctx : ∀ n, lctxty (rty n)) (n : Nat) :
+    HEq (restoreAtDep (.succ pos) restoreDep (pushLCtxDep x lctx) n) (pushLCtxDep x (restoreAtDep pos restoreDep lctx) n) :=
+    match pos, n with
+    | 0,          0        => HEq.rfl
+    | 0,          .succ _  => HEq.rfl
+    | .succ _,    0        => HEq.rfl
+    | .succ pos', .succ n' => by
+      apply HEq.trans (restoreAtDep.succ_succ (Nat.succ pos') restoreDep (pushLCtxDep x lctx) n')
+      rw [pushLCtxDep.succ]; rw [pushLCtxDep.succ_Fn]
 
-def pushLCtxAtDep.equivFn {rty : Nat → α} {lctxty : α → Sort u}
-  (lctx : ∀ n, lctxty (rty n)) {xty : α} (x : lctxty xty) (pos : Nat) :
-    HEq (pushLCtxAtDepRec lctx x pos) (pushLCtxAtDep lctx x pos) :=
-    HEq.funext _ _ (fun n => pushLCtxAtDep.equiv lctx x pos n)
+  theorem restoreAtDep.succ_pushLCtxDep_Fn
+    (restore : ∀ {α}, (Nat → α) → (Nat → α))
+    (restoreDep : ∀ {α} {rty : Nat → α} {lctxty : α → Sort u}, (∀ n, lctxty (rty n)) → ∀ n, lctxty ((restore rty) n))
+    {rty : Nat → α} {lctxty : α → Sort u} {xty : α} (x : lctxty xty) (pos : Nat)
+    (lctx : ∀ n, lctxty (rty n)) :
+    HEq (restoreAtDep (.succ pos) restoreDep (pushLCtxDep x lctx)) (pushLCtxDep x (restoreAtDep pos restoreDep lctx)) :=
+    HEq.funext _ _ (fun n => restoreAtDep.succ_pushLCtxDep restore restoreDep x pos lctx n)
 
-def pushLCtxAtDepRec.comm {α : Sort w} {β : α → Sort x} {rty : Nat → α} {lctxty : α → Sort u}
-  (f : ∀ (x : α), lctxty x → β x) (lctx : ∀ n, lctxty (rty n))
-  {xty : α} (x : lctxty xty) : (pos : Nat) → (n : Nat) →
-    f _ (pushLCtxAtDepRec lctx x pos n) = pushLCtxAtDepRec (lctxty:=β) (fun n => f _ (lctx n)) (f xty x) pos n
-| 0 => fun _ => pushLCtxDep.comm _ _ _ _
-| pos' + 1 => fun n =>
-  match n with
-  | 0 => rfl
-  | n' + 1 => pushLCtxAtDepRec.comm f (fun n => lctx (Nat.succ n)) x pos' n'
+  def covPairDep
+    (f : Nat → Nat) (restore : ∀ {α}, (Nat → α) → (Nat → α))
+    (restoreDep : ∀ {α} {rty : Nat → α} {lctxty : α → Sort u}, (∀ n, lctxty (rty n)) → ∀ n, lctxty ((restore rty) n)) :=
+    covPair f restore ∧
+      ∀ {α} {rty : Nat → α} {lctxty : α → Sort u} (lctx : ∀ n, lctxty (rty n)) (n : Nat),
+        HEq (@restoreDep _ rty lctxty lctx (f n)) (lctx n)
 
-def pushLCtxAtDepRec.nonDep {rty : Nat → α} {lctxty : Sort u}
-  (lctx : Nat → lctxty) {xty : α} (x : lctxty) : (pos n : Nat) →
-  @pushLCtxAtDepRec _ rty (fun _ => lctxty) lctx xty x pos n = pushLCtxAtRec lctx x pos n
-| 0 => fun _ => rfl
-| .succ pos' => fun n =>
-  match n with
-  | 0 => rfl
-  | .succ n' => pushLCtxAtDepRec.nonDep (fun n => lctx (.succ n)) x pos' n'
+  def covPairDepAt
+    (f : Nat → Nat) (restore : ∀ {α}, (Nat → α) → (Nat → α))
+    (restoreDep : ∀ {α} {rty : Nat → α} {lctxty : α → Sort u}, (∀ n, lctxty (rty n)) → ∀ n, lctxty ((restore rty) n)) :=
+    covPairAt f restore ∧
+      ∀ {α} (pos : Nat) {rty : Nat → α} {lctxty : α → Sort u} (lctx : ∀ n, lctxty (rty n)) (n : Nat),
+        HEq (restoreAtDep pos restoreDep (rty:=rty) lctx (mapAt pos f n)) (lctx n)
 
-def pushLCtxAtDepRec.absorbAux {rty : Nat → α} {lctxty : α → Sort u}
-  (lctx : ∀ n, lctxty (rty n)) {xty : α} (x : lctxty xty) :
-  (pos : Nat) → (n : Nat) → HEq
-    (@pushLCtxAtDepRec _ rty lctxty lctx _ x pos n)
-    (@pushLCtxAtDepRec _ (lctxty ∘ rty) id lctx _ x pos n)
-| 0 => fun _ => pushLCtxDep.absorbAux _ _ _
-| pos' + 1 => fun n =>
-  match n with
-  | 0 => HEq.refl _
-  | n' + 1 => pushLCtxAtDepRec.absorbAux (fun n => lctx (.succ n)) x pos' n'
+  theorem covPairDepAt.ofCovPairDep (cpd : covPairDep f restore restoreDep) :
+    covPairDepAt f restore restoreDep := by
+    apply And.intro
+    case left => exact covPairAt.ofCovPair cpd.left
+    case right =>
+      intros α pos rty lctxty lctx n
+      dsimp [restoreAt, restoreAtDep, mapAt]
+      match h : pos.ble n with
+      | true =>
+        dsimp;
+        have heq : Nat.ble pos (f (n - pos) + pos) = true := by
+          apply Nat.ble_eq_true_of_le;
+          apply Nat.le_add_left
+        have hle := Nat.le_of_ble_eq_true h
+        rw [heq]; dsimp
+        rw [Nat.add_sub_assoc .refl]; rw [Nat.sub_self]; dsimp
+        apply HEq.trans (b:=lctx (n - pos + pos))
+        case h₁ => apply cpd.right
+        case h₂ => rw [Nat.sub_add_cancel hle]
+      | false => dsimp; rw [h]
 
-theorem pushLCtxAtDepRec.absorb {rty : Nat → α} {lctxty : α → Sort u}
-  (lctx : ∀ n, lctxty (rty n)) {xty : α} (x : lctxty xty) (pos : Nat) :
-  HEq (@pushLCtxAtDepRec _ rty lctxty lctx _ x pos) (@pushLCtxAtDepRec _ (lctxty ∘ rty) id lctx _ x pos) :=
-  HEq.funext _ _ (pushLCtxAtDepRec.absorbAux _ _ _)
-
--- Surprisingly, this is definitionally equal
-def pushLCtxDep_pushLCtxAtDepRec {rty : Nat → α} {lctxty : α → Sort u}
-  (lctx : ∀ n, lctxty (rty n)) {xty : α} (x : lctxty xty) {yty : α} (y : lctxty yty) (pos : Nat) :
-  pushLCtxDep (pushLCtxAtDepRec lctx x pos) y = pushLCtxAtDepRec (pushLCtxDep lctx y) x (Nat.succ pos) := rfl
-
-def popLCtx (lctx : Nat → α) := fun n => lctx (n + 1)
-
-def popLCtx.comm (f : α → β) (lctx : Nat → α) :
-  (n : Nat) → f (popLCtx lctx n) = popLCtx (f ∘ lctx) n := fun _ => rfl
-
-def popLCtx.commFn (f : α → β) (lctx : Nat → α) :
-  (fun n => f (popLCtx lctx n)) = (fun n => popLCtx (f ∘ lctx) n) := rfl
-
-def popLCtxDep {rty : Nat → α} {lctxty : α → Sort u}
-  (lctx : ∀ n, lctxty (rty n)) : ∀ n, lctxty (popLCtx rty n) :=
-  fun n => lctx (n + 1)
-
-def popLCtxDep.comm {α : Sort w} {β : α → Sort x} {rty : Nat → α} {lctxty : α → Sort u}
-  (f : ∀ (x : α), lctxty x → β x) (lctx : ∀ n, lctxty (rty n)) (n : Nat) :
-  f _ (popLCtxDep lctx n) = popLCtxDep (lctxty:=β) (fun n => f _ (lctx n)) n := rfl
-
-def popLCtxDep.absorbAux {rty : Nat → α} {lctxty : α → Sort u}
-  (lctx : ∀ n, lctxty (rty n)) (n : Nat) : HEq
-    (@popLCtxDep _ rty lctxty lctx n)
-    (@popLCtxDep _ (lctxty ∘ rty) id lctx n) := HEq.refl _
-
-theorem popLCtxDep.absorb {rty : Nat → α} {lctxty : α → Sort u} (lctx : ∀ n, lctxty (rty n)) :
-  HEq (@popLCtxDep _ rty lctxty lctx) (@popLCtxDep _ (lctxty ∘ rty) id lctx) :=
-  HEq.funext _ _ (popLCtxDep.absorbAux _)
-
-def popLCtxAt (lctx : Nat → α) (pos n : Nat) :=
-  match pos.ble n with
-  | true => lctx (.succ n)
-  | false => lctx n
-
-def popLCtxAtRec (lctx : Nat → α) (pos : Nat) := 
-  match pos with
-  | 0 => popLCtx lctx
-  | pos' + 1 => fun n =>
-    match n with
-    | 0 => lctx 0
-    | n' + 1 => popLCtxAtRec (fun n => lctx (Nat.succ n)) pos' n'
-
-theorem popLCtxAt.equiv (lctx : Nat → α) (pos n : Nat) :
-  popLCtxAtRec lctx pos n = popLCtxAt lctx pos n := by
-  revert lctx n; induction pos <;> intro lctx n
-  case zero =>
-    cases n <;> rfl
-  case succ pos' IH =>
-    cases n
-    case zero => rfl
-    case succ n' => exact (IH (fun n => lctx (.succ n)) n')
-
-def popLCtxAtRec.comm (lctx : Nat → α) (f : α → β) (pos : Nat) :
-  (n : Nat) → f (popLCtxAtRec lctx pos n) = popLCtxAtRec (f ∘ lctx) pos n :=
-  match pos with
-  | 0 => fun _ => rfl
-  | pos' + 1 => fun n =>
-    match n with
-    | 0 => rfl
-    | n' + 1 => popLCtxAtRec.comm (fun n => lctx (.succ n)) f pos' n'
-
-def popLCtxAtRec.commFn (lctx : Nat → α) (f : α → β) (pos : Nat) :
-  (fun n => f (popLCtxAtRec lctx pos n)) = (fun n => popLCtxAtRec (f ∘ lctx) pos n) :=
-  funext (popLCtxAtRec.comm lctx f pos)
-
-def popLCtxAtDep {rty : Nat → α} {lctxty : α → Sort u}
-  (lctx : ∀ n, lctxty (rty n)) (pos : Nat) (n : Nat) : lctxty (popLCtxAt rty pos n) := by
-  dsimp [popLCtxAt]
-  match pos.ble n with
-  | true => exact lctx (.succ n)
-  | false => exact lctx n
-
-def popLCtxAtDepRec {rty : Nat → α} {lctxty : α → Sort u}
-  (lctx : ∀ n, lctxty (rty n)) : (pos : Nat) → (n : Nat) → lctxty (popLCtxAtRec rty pos n)
-| 0 => popLCtxDep lctx
-| pos' + 1 => fun n =>
-  match n with
-  | 0 => lctx 0
-  | n' + 1 => popLCtxAtDepRec (fun n => lctx (Nat.succ n)) pos' n'
-
-def popLCtxAtDepRec.absorbAux {rty : Nat → α} {lctxty : α → Sort u}
-  (lctx : ∀ n, lctxty (rty n)) : (pos : Nat) → (n : Nat) → HEq
-    (@popLCtxAtDepRec _ rty lctxty lctx pos n)
-    (@popLCtxAtDepRec _ (lctxty ∘ rty) id lctx pos n)
-| 0 => fun _ => HEq.refl _
-| pos' + 1 => fun n =>
-  match n with
-  | 0 => HEq.refl _
-  | n' + 1 => popLCtxAtDepRec.absorbAux (fun n => lctx (.succ n)) pos' n'
-
-def popLCtxAtDepRec.absorbAux' {rty : Nat → α} {lctxty : α → Sort u}
-  (lctx : ∀ n, lctxty (rty n)) (pos : Nat) (n : Nat) : HEq
-    (@popLCtxAtDepRec _ rty lctxty lctx pos n)
-    (@popLCtxAtDepRec _ id (lctxty ∘ rty) lctx pos n) :=
-  HEq.trans
-    (b := @popLCtxAtDepRec _ (lctxty ∘ rty) id lctx pos n)
-    (popLCtxAtDepRec.absorbAux lctx pos n)
-    (HEq.symm (@popLCtxAtDepRec.absorbAux _ id (lctxty ∘ rty) lctx pos n))
-
-def popLCtxAtDepRec.absorb {rty : Nat → α} {lctxty : α → Sort u} (lctx : ∀ n, lctxty (rty n)) (pos : Nat):
-  HEq (@popLCtxAtDepRec _ rty lctxty lctx pos) (@popLCtxAtDepRec _ (lctxty ∘ rty) id lctx pos) :=
-  HEq.funext _ _ (popLCtxAtDepRec.absorbAux _ _)
-
-def popLCtxAtDepRec.comm {α : Sort w} {β : α → Sort x} {rty : Nat → α} {lctxty : α → Sort u}
-  (f : ∀ (x : α), lctxty x → β x) (lctx : ∀ n, lctxty (rty n)) :
-  (pos : Nat) → (n : Nat) → f _ (popLCtxAtDepRec lctx pos n) = popLCtxAtDepRec (lctxty:=β) (fun n => f _ (lctx n)) pos n
-| 0 => fun _ => rfl
-| pos' + 1 => fun n =>
-  match n with
-  | 0 => rfl
-  | n' + 1 => popLCtxAtDepRec.comm f (fun n => lctx (Nat.succ n)) pos' n'
-
-def popLCtxAtRec.commDep
-  {β : α → Sort u} (lctx : Nat → α) (f : ∀ (x : α), β x) :
-  (pos n : Nat) → f (popLCtxAtRec lctx pos n) = popLCtxAtDepRec (fun n => f (lctx n)) pos n
-| 0 => fun _ => rfl
-| pos' + 1 => fun n =>
-  match n with
-  | 0 => rfl
-  | n' + 1 => popLCtxAtRec.commDep (fun n => lctx (.succ n)) f pos' n'
- 
--- #reduce fun lctx => popLCtxAtRec lctx 3 4
-
-def push_pop_eq (lctx : Nat → α) :
-  pushLCtx (popLCtx lctx) (lctx 0) = lctx := by
-  apply funext
-  intro n; cases n <;> rfl
-
-def popAtRec_pushAtRec_eq (lctx : Nat → α) (x : α) :
-  (pos : Nat) → (n : Nat) → popLCtxAtRec (pushLCtxAtRec lctx x pos) pos n = lctx n
-| 0 => fun _ => rfl
-| pos' + 1 => fun n =>
-  match n with
-  | 0 => rfl
-  | n' + 1 => popAtRec_pushAtRec_eq (fun n => lctx (Nat.succ n)) x pos' n'
-
-def popAtDepRec_pushAtDepRec_eq
-  {α : Sort w} {rty : Nat → α} {lctxty : α → Sort u}
-  (lctx : ∀ n, lctxty (rty n)) {xty : α} (x : lctxty xty) : (pos n : Nat) →
-  HEq (@popLCtxAtDepRec _ (pushLCtxAtRec rty xty pos) lctxty
-        (@pushLCtxAtDepRec _ rty lctxty lctx xty x pos) pos n
-      )
-      (lctx n)
-| 0 => fun _ => HEq.rfl
-| pos' + 1 => fun n =>
-  match n with
-  | 0 => HEq.rfl
-  | n' + 1 => @popAtDepRec_pushAtDepRec_eq _ _ lctxty (fun n => lctx (Nat.succ n)) _ x pos' n'
-
-def popLCtxsAt (lctx : Nat → α) (lvl pos n : Nat) :=
-  match pos.ble n with
-  | true => lctx (Nat.add n lvl)
-  | false => lctx n
-
-def popLCtxsAt.comm (f : α → β) (lctx : Nat → α) (lvl : Nat) (pos n : Nat) :
-  f (popLCtxsAt lctx lvl pos n) = popLCtxsAt (f ∘ lctx) lvl pos n := by
-  dsimp [popLCtxsAt]
-  match Nat.ble pos n with
-  | true => rfl
-  | false => rfl
-
-def popLCtxsAt.succ_l (lctx : Nat → α) (lvl : Nat) (pos n : Nat) :
-  popLCtxsAt lctx (.succ lvl) pos n = popLCtxsAt (popLCtxAt lctx pos) lvl pos n := by
-  dsimp [popLCtxsAt, popLCtxAt]
-  match h : Nat.ble pos n with
-  | true =>
-    dsimp
-    have leAdd' := Nat.le_trans (Nat.le_of_ble_eq_true h) (Nat.le_add_right _ lvl)
-    have bleAdd' := Nat.ble_eq_true_of_le leAdd'
-    rw [bleAdd']; rfl
-  | false => rfl
-
-def popLCtxsAt.succ_r (lctx : Nat → α) (lvl : Nat) (pos n : Nat) :
-  popLCtxsAt lctx (.succ lvl) pos n = popLCtxAt (popLCtxsAt lctx lvl pos) pos n := by
-  dsimp [popLCtxsAt, popLCtxAt]
-  match h : Nat.ble pos n with
-  | true =>
-    dsimp
-    dsimp
-    have leAdd' := Nat.le_trans (Nat.le_of_ble_eq_true h) (Nat.le_add_right _ 1)
-    have bleAdd' := Nat.ble_eq_true_of_le leAdd'
-    rw [bleAdd', Nat.succ_add]; rfl
-  | false => rfl
-
-def popLCtxsAt.one (lctx : Nat → α) :
-  popLCtxsAt lctx 1 = popLCtxAt lctx := rfl
-
-@[reducible] def pushLCtxs (lctx : Nat → α) (xs : List α) (n : Nat) : α :=
-  match h : Nat.blt n xs.length with
-  | true  => xs[n]'(Nat.le_of_ble_eq_true h)
-  | false => lctx (n - xs.length)
+end generic
 
 end Auto.Embedding
